src/program_logic/distributed_weakestpre.v
@@ -2,24 +2,36 @@ From iris.proofmode Require Import tactics.
 From iris.algebra Require Import gmap auth agree gset coPset.
 From Perennial.base_logic.lib Require Import wsat.
 From Perennial.program_logic Require Export weakestpre.
-From Perennial.program_logic Require Export crash_lang crash_weakestpre recovery_weakestpre.
+From Perennial.program_logic Require Export crash_lang dist_lang crash_weakestpre recovery_weakestpre.
 Import uPred.
 
 Set Default Proof Using "Type".
 
 (*** Distributed WP ***)
 
+Class groveG (Λ : language) (CS: crash_semantics Λ) (Σ : gFunctors) := GroveG {
+  grove_global_state_interp : global_state Λ → nat → list (observation Λ) → iProp Σ;
+  grove_num_laters_per_step : nat → nat;
+  grove_invG :> invG Σ;
+}.
+
 Section wpd.
+Context `{gG: !groveG Λ CS Σ}.
 Context `{pG: !perennialG Λ CS T Σ}.
 
+(*
 Definition equal_global_interp ct1 ct2 :=
   @global_state_interp _ _(perennial_irisG (fst ct1) (snd ct1)) =
   @global_state_interp _ _(perennial_irisG (fst ct2) (snd ct2)).
+*)
 
-(* maybe the global interp should be a parameter that they are all equal to,
-   rather than saying they're all equal? *)
+Definition equal_global_inG ct :=
+  @global_state_interp _ _(perennial_irisG (fst ct) (snd ct)) = grove_global_state_interp ∧
+  @num_laters_per_step _ _(perennial_irisG (fst ct) (snd ct)) = grove_num_laters_per_step ∧
+  @iris_invG _ _ (perennial_irisG (fst ct) (snd ct)) = grove_invG.
+
 Definition wpd (k : nat) (E: coPset) (cts: list (crashG Σ * pbundleG T Σ)) (es: list (expr Λ)) :=
- (⌜ ∀ ct1 ct2, ct1 ∈ cts → ct2 ∈ cts → equal_global_interp ct1 ct2 ⌝ ∧
+ (⌜ ∀ ct, ct ∈ cts → equal_global_inG ct ⌝ ∧
  [∗ list] i↦ct;e ∈ cts;es, ∃ Φ Φrx Φinv, wpr NotStuck k (fst ct) (snd ct) E e e Φ Φinv Φrx)%I.
 
 End wpd.
